Makefile
@@ -1,0 +1,16 @@
+
+html	: doc/EnumeratingTheRationals.html
+latex	: doc/EnumeratingTheRationals.tex
+pdf		: doc/EnumeratingTheRationals.pdf
+
+doc:
+	mkdir -p doc
+	
+doc/EnumeratingTheRationals.html: doc EnumeratingTheRationals.v
+	coqdoc --html --no-index -s -d doc EnumeratingTheRationals.v
+	
+doc/EnumeratingTheRationals.tex	: doc EnumeratingTheRationals.v
+	coqdoc --latex --no-index -s -d doc EnumeratingTheRationals.v
+	
+doc/EnumeratingTheRationals.pdf	: doc/EnumeratingTheRationals.tex
+	pdflatex doc/EnumeratingTheRationals.tex
